polymorphism/Proofs/Records/Examples.v
@@ -1,0 +1,54 @@
+Require Import String.
+Require Import Coq.Structures.Equalities.
+Require Import Coq.MSets.MSetInterface.
+Require Import Arith.
+Require Import Setoid.
+Require Import Coq.Program.Equality.
+Require Import SystemF.
+Require Import Extended.
+
+Module MExamples
+       (Import VarTyp : UsualDecidableTypeFull)
+       (Import set : MSetInterface.S).
+
+Module MExtended := MExtended(VarTyp)(set).
+Export MExtended.
+
+(*** Records ***)
+
+(* { x := 3 }.x : Int *)
+
+Parameter x : var.
+Definition RecX := PRec x (PLit 3).
+Theorem ex1 : exists c, has_type_source_alg nil (PProjR RecX x) Inf PInt c.
+  eexists; unfold RecX. eauto.
+Defined.
+
+(* ({ x := 3 } ,, { y := 4 }).x : Int *) (* needs annotation *)
+
+Parameter y : var.
+Definition RecY := PRec y (PLit 4).
+Definition RecXTy := (Rec x PInt).
+Theorem ex2 :
+  x <> y ->
+  exists c, has_type_source_alg nil (PProjR (PAnn (PMerge RecX RecY) RecXTy) x) Inf PInt c.
+  eexists; unfold RecX, RecY, RecXTy.
+  apply ATyProjR.
+  apply ATyAnn.
+  apply ATySub with (A := And (Rec x PInt) (Rec y PInt)); eauto.
+  apply ATyMerge; eauto.
+Defined.
+
+(* ({ x := 3 } ,, { x := () }).x : Int *) (* needs annotation *)
+
+Definition RecX' := PRec x PUnit.
+Theorem ex3 :
+  exists c, has_type_source_alg nil (PProjR (PAnn (PMerge RecX RecX') RecXTy) x) Inf PInt c.
+  eexists; unfold RecX, RecX', RecXTy.
+  apply ATyProjR.
+  apply ATyAnn.
+  apply ATySub with (A := And (Rec x PInt) (Rec x Top)); eauto.
+  apply ATyMerge; eauto.
+Defined.
+
+End MExamples.
